LEAN/Tutorial/Lean/ACLS.lean
@@ -1,0 +1,437 @@
+-- source:  https://cpr.heart.org/en/resuscitation-science/cpr-and-ecc-guidelines/algorithms
+-- blue action box = ArrestState + actions
+-- red decision diamond = match on patient observation
+-- arrow = nextState branch
+-- loop back arrow = transition to earlier states
+
+/--
+this funciton returns true if any of the conditions in the list are true
+it returns false if and only iff all conditions are explicitly false
+it will return unknown otherwise -/
+def optionOrList : List (Option Bool) → Option Bool
+  | [] => some false
+  | xs =>
+      if xs.any (· == some true) then
+        some true
+      else if xs.any (· == none) then
+        none
+      else
+        some false
+
+/--
+this function returns true if and only if all the conditions are true
+it returns false if any of the conditions are false
+and unknown (none) otherwise -/
+def optionAndList : List (Option Bool) → Option Bool
+  | [] => some true
+  | xs =>
+      if xs.any (· == some false) then
+        some false
+      else if xs.any (· == none) then
+        none
+      else
+        some true
+
+/--
+helper function that takes a decidable equation and a possible value for it
+and returns if the equation takes on that value-/
+def optionEq [DecidableEq α] (x : Option α) (y : α) : Option Bool :=
+  match x with
+  | some z => some (z = y)
+  | none => none
+
+/--
+helper function for determining if a given condition takes a value greater
+than a specific given natural number-/
+def optionGt (x : Option Nat) (n : Nat) : Option Bool :=
+  match x with
+  | some m => some (m > n)
+  | none => none
+
+/--
+helper function for determining if a given condition takes a value less
+than a sprcific given natural number -/
+def optionLt (x : Option Nat) (n : Nat) : Option Bool :=
+  match x with
+  | some m => some (m < n)
+  | none => none
+
+/--
+helper function for determining if a given condition that takes a list contains
+a specific given string-/
+def optionContains [DecidableEq α] (xs : Option (List α)) (x : α) : Option Bool :=
+  match xs with
+  | some ys => some (x ∈ ys)
+  | none => none
+
+def optionNot : Option Bool → Option Bool
+| some true => some false
+| some false => some true
+| none => none
+
+inductive Rhythm
+  | VentricularFibrillation
+  | PulselessVT
+  | Asystole
+  | PulselessElectricalActivity
+deriving DecidableEq, Repr
+
+inductive Pulse where
+  | Present
+  | Absent
+deriving DecidableEq, Repr
+
+def Rhythm.isShockable : Rhythm → Prop
+| .VentricularFibrillation => True
+| .PulselessVT             => True
+| _                        => False
+
+def Rhythm.isShockableBool : Rhythm → Bool
+| .VentricularFibrillation => true
+| .PulselessVT            => true
+| _                       => false
+
+
+-- types of vascular access, (TODO: IV is preferred, if not, then IO)
+inductive VascularAccess where
+  | None
+  | IV_IO
+deriving DecidableEq, Repr
+
+inductive Airway where
+  | Basic
+  | Advanced
+deriving DecidableEq, Repr
+
+
+-- Timer kinds to evaluate different procedures
+inductive TimerKind where
+  | CPR
+  | Epinephrine
+  | Antiarrhythmic
+deriving DecidableEq, Repr
+
+structure Timer where
+  duration: Nat
+  type: TimerKind
+deriving DecidableEq, Repr
+
+-- possible states represented in the algorithm. numbers match the AHA algorithm
+inductive ArrestState where
+  | InitialAssessment
+  | InitialACLS
+  | CPR
+  | RhythmAnalysis
+  | ROSC
+  | Terminated
+deriving DecidableEq, Repr
+
+-- possible events that deteremine the decision tree branch
+inductive Event
+| CPRStarted
+| CPRTimerStarted
+| CPRDone
+| EntireACLSCompleted
+| RhythmObserved (r : Rhythm)
+| ShockDelivered
+| EpinephrineGiven
+| EpinephrineTimerStarted
+| AmiodaroneOrLidocaineGiven
+| AmidaroneLidocaineTimerStarted
+| PulseDetected
+| NoPulseDetected
+| IV_IOEstablished
+| DefibrillatorAttached
+| MonitorAttached
+| AllEquipmentAttached
+| AirwayPlaced
+| TimerExpired (t: TimerKind)
+| PostCPRDone
+deriving DecidableEq, Repr
+
+-- possible actions the professional can take
+inductive Action where
+  | StartHighQualityCPR
+  | AnalyzeRhythm
+  | CheckPulse
+  | DeliverShock
+  | AttachMonitor
+  | AttachDefibrillator
+  | ObtainIVIO
+  | AdministerEpinephrine
+  | AdministerAmiodaroneOrLidocaine
+  | GiveOxygen
+  | PlaceAdvancedAirway
+  | UseCapnography
+  | TreatReversibleCauses
+  | FinishTreatment
+deriving DecidableEq, Repr
+
+-- could also divide these into PatientObservatin, TreatmentHistory, Equipment, etc.
+structure ArrestPatient where
+  rhythm : Option Rhythm
+  pulse : Option Pulse --Present or Absent
+
+  shockCount : Nat
+  cprCycle: Nat
+
+  epinephrineCount : Nat
+  amiodaroneOrLidocaineCount : Nat
+
+  monitorAttached : Bool
+  defibrillatorAttached : Bool
+
+  vascularAccess : VascularAccess
+
+  airway: Airway
+
+  timers : List Timer
+
+  latestEvent : Option Event
+deriving DecidableEq, Repr
+
+
+-- structure Reminder where
+--   message : String
+--   -- (TODO) remainingSeconds: Option Nat
+-- deriving Repr
+
+structure ProtocolOutput where
+  actions : List Action
+  reminders : List String
+deriving DecidableEq, Repr
+
+
+def ACLSOutput
+  (s : ArrestState)
+  (p : ArrestPatient)
+  : ProtocolOutput :=
+  match s with
+  | .InitialAssessment =>
+      match p.pulse with
+      | Pulse.Present =>
+          { actions := [.FinishTreatment]
+            reminders := ["Ensure patient is good to leave"]}
+      | Pulse.Absent =>
+          { actions := [.StartHighQualityCPR]
+            reminders := [ "Start CPR immedietly"]}
+      | none =>
+          { actions := [.CheckPulse]
+            reminders := [ "Check pulse and breathing for 5-10 seconds"] }
+    | .InitialACLS =>
+      { actions :=
+          [ .GiveOxygen
+          , .AttachMonitor
+          , .AttachDefibrillator
+          , .ObtainIVIO ]
+        reminders :=
+          [ "Perform CPR for 2 minutes"
+          , "Maintain compression rate 100-120/min"
+          , "Allow full chest recoil by pushing down at least 5cm (2inch)"
+          , "Give enough air for visible chest rise" ] }
+
+-- change this CPR to be CPRShockable and CPRNonShockable
+  | .CPR =>
+      let baseActions := [ Action.StartHighQualityCPR ]
+      let baseReminders :=
+      [ "Perform CPR for 2 minutes"
+      , "Maintain compression rate 100-120/min"
+      , "Allow full chest recoil by pushing down at least 5cm (2 inch)"
+      , "Give enough air for visible chest rise"
+      , "Change compressor every 2 minutes"
+      ]
+      let rhythmActions :=
+        match p.rhythm with
+        | none => [Action.AnalyzeRhythm]
+        | some _ => []
+      let epiActions :=
+        if p.shockCount >= 2 && p.shockCount % 2 == 0 then
+          [ Action.AdministerEpinephrine ]
+        else []
+      let antiArrhythmicAction :=
+        if p.shockCount >= 3 && p.shockCount % 2 == 1 then
+          match p.rhythm with
+          | some r =>
+              if r.isShockableBool then
+                [ Action.AdministerAmiodaroneOrLidocaine ]
+              else []
+          | none => []
+        else []
+
+        let actions :=
+          baseActions
+          ++ epiActions
+          ++ antiArrhythmicAction
+          ++ rhythmActions
+          ++ [Action.PlaceAdvancedAirway, Action.UseCapnography]
+
+        let reminders :=
+          baseReminders
+          ++ (if Action.AdministerEpinephrine ∈ actions then
+                ["Administer 1 mg epinephrine. Next one coming up in 3-5 minutes."]
+              else
+                [])
+          ++ (if Action.AdministerAmiodaroneOrLidocaine ∈ actions && p.amiodaroneOrLidocaineCount = 0 then
+                ["Administer the first dose of amiodarone 300 mg IV push or lidocaine 1 to 1.5 mg/kg"]
+              else if Action.AdministerAmiodaroneOrLidocaine ∈ actions && p.amiodaroneOrLidocaineCount > 0 then
+                ["Administer a lower dose of amidoarone,150 mg IV push or lidocanine 0.5 to 0.75 mg/kg"]
+              else
+                [])
+          ++ (if Action.AnalyzeRhythm ∈ actions then
+                ["Analyze the Rhythm to detemine shockability immedietly"]
+              else
+                ["Next rhythm analysis when CPR timer expires"])
+          ++ (if p.airway == Airway.Advanced then
+                ["Since advanced airway is placed, give breaths every 6 seconds, while maintaining compressions"]
+              else
+              [])
+        { actions := actions
+          reminders := reminders }
+
+  | .RhythmAnalysis =>
+      match p.rhythm with
+      | some r =>
+          if r.isShockableBool then
+            { actions := [ .DeliverShock ]
+              reminders :=
+                [ "Resume CPR immediately after shock"
+                , "Depending on the defib branch, Monophasic, Zoll, Philips, Stryker/LifePak
+                use 360J, 120J, 150J, 200J respectively. " ] }
+          else
+            { actions :=
+                [ .StartHighQualityCPR
+                , .TreatReversibleCauses ]
+              reminders :=
+                [ "Administer epinephrine as early as possible" ] }
+
+      | none =>
+          { actions := [ .AnalyzeRhythm ]
+            reminders := [] }
+
+  | .ROSC =>
+      { actions := []
+        reminders := [ "Begin post-cardiac arrest care" ] }
+
+  | .Terminated =>
+      { actions := []
+        reminders := [] }
+
+
+def updateState
+  (state : ArrestState)
+  (patient : ArrestPatient)
+  (e : Event)
+  : ArrestState × ArrestPatient :=
+  match e with
+  | .CPRStarted =>
+
+      let updated := {patient with
+      latestEvent := Event.CPRStarted
+      timers :=
+        patient.timers ++
+        [
+          {
+            duration := 120,
+            type := TimerKind.CPR
+          }
+        ]
+      }
+      if state == .InitialAssessment then
+      (.InitialACLS, updated)
+      else
+      (.CPR, updated)
+  | .EntireACLSCompleted =>
+      (.Terminated, {patient with latestEvent := Event.EntireACLSCompleted})
+  | .RhythmObserved r =>
+      let updated := { patient with
+                        rhythm := some r
+                        latestEvent := Event.RhythmObserved r}
+      (.RhythmAnalysis, updated)
+  | .ShockDelivered =>
+      let updated :=
+        { patient with
+            shockCount := patient.shockCount + 1
+            latestEvent := Event.ShockDelivered}
+      (.CPR, updated)
+  | .EpinephrineGiven =>
+      let updated :=
+        { patient with
+            epinephrineCount := patient.epinephrineCount + 1
+            timers :=
+              patient.timers ++
+              [
+                {
+                  duration := 240,
+                  type := TimerKind.Epinephrine
+                }
+              ]
+        }
+    (.RhythmAnalysis, updated)
+  | .AmiodaroneOrLidocaineGiven =>
+      let updated :=
+        { patient with
+            amiodaroneOrLidocaineCount :=
+              patient.amiodaroneOrLidocaineCount + 1
+            timers :=
+              patient.timers ++
+              [
+                {
+                  duration := 240,
+                  type := TimerKind.Antiarrhythmic
+                }
+              ]
+            latestEvent := Event.AmiodaroneOrLidocaineGiven}
+      (.RhythmAnalysis, updated)
+  | .PulseDetected =>
+      let updated := { patient with pulse := some Pulse.Present
+                                    latestEvent := Event.PulseDetected }
+      (.ROSC, updated)
+  | .NoPulseDetected =>
+      let updated := { patient with pulse := some Pulse.Absent
+                                    latestEvent := Event.NoPulseDetected}
+      (.InitialAssessment, updated)
+  | .IV_IOEstablished =>
+    let updated := { patient with vascularAccess := VascularAccess.IV_IO
+                                  latestEvent := Event.IV_IOEstablished}
+    (state, updated)
+  | .DefibrillatorAttached =>
+      let updated := { patient with defibrillatorAttached := true
+                                    latestEvent := Event.DefibrillatorAttached}
+      (state, updated)
+  | .MonitorAttached =>
+      let updated := { patient with monitorAttached := true
+                                    latestEvent := Event.MonitorAttached}
+      (state, updated)
+  | .AllEquipmentAttached =>
+      let updated := { patient with
+        defibrillatorAttached := true
+        monitorAttached := true
+        vascularAccess := VascularAccess.IV_IO
+        latestEvent := Event.AllEquipmentAttached
+      }
+      (state, updated)
+  | .CPRDone =>
+      let updated := { patient with cprCycle := patient.cprCycle + 1
+                                    latestEvent := Event.CPRDone}
+      (.RhythmAnalysis, updated)
+  | .AirwayPlaced =>
+      let updated := { patient with airway := Airway.Advanced
+                                    latestEvent := Event.AirwayPlaced}
+      (state, updated)
+  | .TimerExpired timerKind =>
+      (state,
+        { patient with
+            timers :=
+              patient.timers.filter
+                (fun t => t.type != timerKind)
+            latestEvent := Event.TimerExpired timerKind
+        })
+  | .PostCPRDone =>
+    (.Terminated, { patient with latestEvent := Event.PostCPRDone})
+
+  | .CPRTimerStarted =>
+    (state, { patient with latestEvent := some Event.CPRTimerStarted})
+  | .EpinephrineTimerStarted =>
+    (state, { patient with latestEvent := some Event.EpinephrineTimerStarted})
+  | .AmidaroneLidocaineTimerStarted =>
+    (state, { patient with latestEvent := some Event.AmidaroneLidocaineTimerStarted})
