LEAN/candidate(template).lean
@@ -1,0 +1,7 @@
+import Tutorial.Lean.moduleTwo
+def User : Patient :=
+{
+}
+
+theorem ValidPlan :
+  TriageAssessment examplePatient = Triage.Priority := by
